src/ppprover.ml
@@ -3,29 +3,41 @@ open Prover
 
 (** val empty_state *)
 
-let lift_printer (p: out_channel -> 'a -> unit)  o v = p o (Annot.elt v)
-
+let lift_printer (p : out_channel -> 'a -> unit) o v = p o (Annot.elt v)
 let string_op = function AND -> "∧" | OR -> "∨" | IMPL -> "→"
+let string_lop = function LAND -> "∧" | LOR -> "∨"
+let op_of_lop = function LAND -> AND | LOR -> OR
 
-let rec output_formula o = function
-  | TT -> output_string o "⊤"
-  | FF -> output_string o "⊥"
-  | AT i -> Printf.fprintf o "p%i" (Uint63.hash i)
-  | OP (op, f1, f2) ->
-    Printf.fprintf o "(%a %s %a)" output_formula f1.HCons.elt (string_op op)
-      output_formula f2.HCons.elt
+let rec output_op_list op o l =
+  match l with
+  | [] ->
+    if op = AND || op = IMPL then output_string o "⊤"
+    else output_string o "⊥"
+  | [f] -> output_formula o f.HCons.elt
+  | f1 :: l ->
+    Printf.fprintf o "%a %s %a" output_formula f1.HCons.elt (string_op op)
+      (output_op_list op) l
+
+and output_formula o = function
+  | LAT i -> Printf.fprintf o "p%i" (Uint63.hash i)
+  | LOP (op, l) -> Printf.fprintf o "(%a)" (output_op_list (op_of_lop op)) l
+  | LIMPL (l, r) ->
+    Printf.fprintf o "(%a → %a)" (output_op_list IMPL) l output_formula
+      r.HCons.elt
 
 let rec output_bformula o = function
   | BTT _ -> output_string o "⊤"
   | BFF _ -> output_string o "⊥"
-  | BAT (_,i) -> Printf.fprintf o "p%i" (Uint63.hash i)
-  | BOP (_,op, f1, f2) ->
-    Printf.fprintf o "(%a.(%i) %s %a.(%i))" output_bformula f1.HCons.elt (Uint63.hash f1.HCons.id) (string_op op)
-      output_bformula f2.HCons.elt (Uint63.hash f2.HCons.id)
+  | BAT (_, i) -> Printf.fprintf o "p%i" (Uint63.hash i)
+  | BOP (_, op, f1, f2) ->
+    Printf.fprintf o "(%a.(%i) %s %a.(%i))" output_bformula f1.HCons.elt
+      (Uint63.hash f1.HCons.id) (string_op op) output_bformula f2.HCons.elt
+      (Uint63.hash f2.HCons.id)
   | BIT _ -> ()
 
-let  output_hbformula o f =
-  Printf.fprintf o "%a.(%i)" output_bformula f.HCons.elt (Uint63.hash f.HCons.id)
+let output_hbformula o f =
+  Printf.fprintf o "%a.(%i)" output_bformula f.HCons.elt
+    (Uint63.hash f.HCons.id)
 
 let output_lit o = function
   | POS p -> Printf.fprintf o "[%a]" output_formula p.HCons.elt
@@ -53,7 +65,7 @@ let output_watched_clause o l =
 let rec unprovable l =
   match l with
   | [] -> false
-  | NEG f :: l -> f.HCons.elt = FF || unprovable l
+  | NEG f :: l -> f.HCons.elt = LOP (LOR, []) || unprovable l
   | POS f :: l -> false
 
 let output_useful_watched_clause o l =
@@ -106,26 +118,28 @@ let output_wneg hm o m =
 let output_state o st =
   Printf.fprintf o "Arrows : %a\n" (output_list output_lit) st.arrows;
   Printf.fprintf o "WNEG : %a\n" (output_wneg st.hconsmap) st.wneg;
-  Printf.fprintf o "Lit : %a\n" ( output_list (lift_printer output_lit)) st.unit_stack;
+  Printf.fprintf o "Lit : %a\n"
+    (output_list (lift_printer output_lit))
+    st.unit_stack;
   Printf.fprintf o "Units : %a\n" (output_units st.hconsmap) st.units;
   Printf.fprintf o "Clauses : %a\n" output_clauses st.clauses
 
-
-
 let output_plit o hm p =
-  PLit.fold (fun () k b ->
+  PLit.fold
+    (fun () k b ->
       match IntMap.get' kInt k hm with
       | None -> failwith "Unknow literal"
-      | Some (b',f) ->
-         match b with
-         | None   -> Printf.fprintf o "Err : %a" output_bformula f
-         | Some b -> Printf.fprintf o "Err : %b %a" b  output_bformula  f) p ()
-             
+      | Some (b', f) -> (
+        match b with
+        | None -> Printf.fprintf o "Err : %a" output_bformula f
+        | Some b -> Printf.fprintf o "Err : %b %a" b output_bformula f ))
+    p ()
+
 (**  *)
 
 (** *)
-
-(*let cnf pol is_classic cp cm ar acc f hf =
+(*
+let cnf pol is_classic cp cm ar acc f hf =
   let x, cl = cnf pol is_classic cp cm ar acc f hf in
   Printf.printf "cnf %a ⊢ %a\n" output_formula f
     (output_list output_useful_watched_clause)
@@ -144,33 +158,39 @@ let output_plit o hm p =
   res
  *)
 (** *)
-
-(*let cnf_hyps b hs st =
+(*
+let cnf_hyps b hs st =
   Printf.printf "cnf_hyps: %a\n" output_literal_list hs;
   cnf_hyps b hs st
  *)
 (** *)
 
-(*let intro_state st f hf =
+(** *)
+(*
+let intro_state st f hf =
   match intro_state st f hf with
-  | None ->
+  | Success _ as r ->
     Printf.printf "intro state ⊢ ⊥ \n";
-    None
-  | Some (st', g) ->
+    r
+  | Progress (st', g) ->
     Printf.printf "intro state ⊢\n%a\n" output_state st';
-    Some (st', g)
+    Progress (st', g)
+  | Fail _ as f ->
+    Printf.printf "intro state ⊢ failure\n";
+    f
  *)
 (** *)
-
-(*let unit_propagation n st concl =
+(*
+let unit_propagation n st concl =
   let res = unit_propagation n st concl in
   ( match res with
-  | Success -> Printf.printf "OK"
-  | OutOfFuel -> Printf.printf "KO"
+  | Success _ -> Printf.printf "OK"
+  | Fail _ -> Printf.printf "KO"
   | Progress st -> Printf.printf "unit_propagation ⊢\n%a\n" output_state st );
   res
  *)
 (** *)
+
 (*let select_clause b l acc k cl =
   let res = select_clause b l acc k cl in
   ( match (acc, res) with
@@ -182,6 +202,7 @@ let output_plit o hm p =
   res
  *)
 (** *)
+
 (*let find_split lit is_bot cl =
   let res = find_split lit is_bot cl in
   ( match res with
@@ -190,6 +211,7 @@ let output_plit o hm p =
   res
  *)
 (** *)
+
 (*let find_arrows st l =
   let res = find_arrows st l in
   Printf.printf "find_arrows %a -> %a\n" (output_list output_lit) l
@@ -201,7 +223,7 @@ let output_plit o hm p =
 let prover_intro p st g =
   let res = prover_intro p st g in
   ( match res with
-  | HasProof _ -> Printf.fprintf stdout "prover ⊢ %a\n" output_oform g
+  | Success _ -> Printf.fprintf stdout "prover ⊢ %a\n" output_oform g
   | _ -> Printf.fprintf stdout "prover ⊬ %a\n" output_oform g );
   flush stdout; res
  *)
