issues/issue_19.v
@@ -1,0 +1,26 @@
+Require Import Lia ZArith.
+Require Import Cdcl.Itauto.
+Open Scope Z_scope.
+
+Unset Lia Cache.
+Set Itauto Theory Time.
+
+Ltac lia_core := xlia zchecker.
+
+Ltac enhanced_lia := Zify.zify; itauto lia_core.
+
+Goal forall (right left : Z) (length_xs v : nat) (x2 x1 : Z) (length_x : nat),
+  (right - left) mod 2 ^ 64 = 8 * Z.of_nat length_xs ->
+  (x2 - x1) mod 2 ^ 64 = 8 * Z.of_nat length_x ->
+  length_x = v ->
+  (x2 - x1) mod 2 ^ 64 <> 0 ->
+  0 <= 8 * Z.of_nat length_x < 2 ^ 64 ->
+  (x1 + (8 * Z.of_nat length_x) mod 2 ^ 64 / 2 ^ 4 * 2 ^ 3 - x1) mod 2 ^ 64 <
+  8 * Z.of_nat length_x.
+Proof.
+  intros.
+  Z.div_mod_to_equations.
+(*  Time lia. (* 16.583 secs *) *)
+  (*  Time itauto lia. (* Theory running time 16.979, Finished transaction in 34.413 secs *)*)
+  Time enhanced_lia. (* Theory running time 19.474, Finished transaction in 41.531 secs *)
+Qed.
