theories/Itauto.v
@@ -7,26 +7,8 @@ Require Import Lia.
 Require Import List.
 Require Import Int63.
 
-
-Notation "'TTT'" := (HCons.mk _ _ TT).
-Notation "'FFF'" := (HCons.mk _ _ FF).
-Notation "A _/\_ B" := (HCons.mk _ _ (OP AND A B)) (at level 80).
-Notation "A _\/_ B" := (HCons.mk _ _ (OP OR A B)) (at level 80).
-Notation "A  -->  B" := (HCons.mk _ _ (OP IMPL A B)) (at level 80).
-Notation "'AT' x" := (HCons.mk _ _ (AT x)) (at level 80).
-
 Declare ML Module "cdcl_plugin".
 Require Import Cdcl.Formula.
-
-
-Ltac elim_nnp :=
-  repeat match goal with
-  | H: context[(?A ?X ?Y -> False) -> False] |- _ =>
-      let prf := constr:(@decP2 _ _ A _ X Y) in
-      rewrite (Decidable.not_not_iff _ prf) in H
-  end.
-
-
 
 Ltac gen_conflicts tac :=
   intros; unfold not in *; unfold iff in *;
@@ -51,7 +33,6 @@ Ltac itauto_use_tauto := constr:(false).
 
 Ltac itauton tac  :=
   gen_conflicts tac ;
-  elim_nnp;
   lazymatch itauto_use_tauto with
   | true => tauto
   | false => run_solver
